Add Π and universes to standard model

coq/cat.v
@@ -13,10 +13,14 @@ Notation "( x ; y ; z ; t ; u ; v )" := (x ; ( y ; (z ; (t ; (u ; v))))).
 Notation "x .π1" := (@projT1 _ _ x) (at level 3, format "x '.π1'").
 Notation "x .π2" := (@projT2 _ _ x) (at level 3, format "x '.π2'").
 
-Definition compose {A B C} (f : B -> C) (g : A -> B) :=
-  fun x => f (g x).
+(* Definition compose {A B C} (f : B -> C) (g : A -> B) :=
+  fun x => f (g x). *)
 
-Notation "f ∘ g" := (compose f g) (at level 0).
+(* Notation "f ∘ g" := (compose f g) (at level 0). *)
+
+Notation "f ∘ g" := (fun x => f (g x)) (at level 20).
+
+Definition id {A} (x : A) : A := x.
 
 Definition Con := Type.
 
@@ -30,13 +34,13 @@ Definition Tm (Γ : Con) (A : Ty Γ) := forall γ : Γ, A γ.
 Definition subsTy {Γ Δ} (σ : Subs Γ Δ) (A : Ty Δ) : Ty Γ :=
   fun γ => A (σ γ).
 
-Notation "A [ σ ]" :=
-  (subsTy σ A)
-  (at level 0).
+Notation "A [ σ ]" := (subsTy σ A) (at level 0).
 
 Definition subsTm {Γ Δ} (σ : Subs Γ Δ) {A} (t : Tm Δ A)
   : Tm Γ A[σ]
   := fun γ => t (σ γ).
+
+Notation "t [ σ ]ᵗ" := (subsTm σ t) (at level 0).
 
 Definition empty : Con :=
   unit.
@@ -44,14 +48,16 @@ Definition empty : Con :=
 Definition cons (Γ : Con) (A : Ty Γ) : Con :=
   ∑ (γ : Γ), A γ.
 
-Definition p {Γ : Con} {A : Ty Γ} : Subs (cons Γ A) Γ :=
+Notation "Γ , A" := (cons Γ A) (at level 20).
+
+Definition p {Γ : Con} {A : Ty Γ} : Subs (Γ, A) Γ :=
   fun '(γ;a) => γ.
 
-Definition q {Γ : Con} {A : Ty Γ} : Tm (cons Γ A) A[p] :=
+Definition q {Γ : Con} {A : Ty Γ} : Tm (Γ, A) A[p] :=
   fun '(γ;a) => a.
 
 Definition scons {Γ Δ} (σ : Subs Γ Δ) {A} (a : Tm Γ A[σ])
-  : Subs Γ (cons Δ A)
+  : Subs Γ (Δ, A)
   := fun γ => (σ γ ; a γ).
 
 Lemma p_scons :
@@ -64,6 +70,82 @@ Qed.
 Lemma q_scons :
   forall Γ Δ (σ : Subs Γ Δ) A (a : Tm Γ A[σ]),
     subsTm (scons σ a) q = a.
+Proof.
+  reflexivity.
+Qed.
+
+(* It supporst Π-types *)
+Definition Π {Γ} (A : Ty Γ) (B : Ty (Γ, A)) : Ty Γ :=
+  fun γ => forall (x : A γ), B (γ ; x).
+
+Definition λ {Γ A B} (b : Tm (Γ, A) B) : Tm Γ (Π A B) :=
+  fun γ => fun (x : A γ) => b (γ ; x).
+
+Definition app {Γ A B} (f : Tm Γ (Π A B)) (u : Tm Γ A) : Tm Γ B[scons id u] :=
+  fun γ => f γ (u γ).
+
+Lemma Πsubs :
+  forall Γ Δ (σ : Subs Γ Δ) (A : Ty Δ) (B : Ty (Δ, A)),
+    (Π A B)[σ] = Π A[σ] B[scons (Γ := Γ,A[σ]) (σ ∘ p) q].
+Proof.
+  reflexivity.
+Qed.
+
+Lemma λsubs :
+  forall Γ Δ (σ : Subs Γ Δ) A B (b : Tm (Δ, A) B),
+    (λ b)[σ]ᵗ = λ (b[scons (Γ := Γ,A[σ]) (σ ∘ p) q]ᵗ).
+Proof.
+  reflexivity.
+Qed.
+
+Lemma app_subs :
+  forall Γ Δ (σ : Subs Γ Δ) A B (f : Tm Δ (Π A B)) (u : Tm Δ A),
+    (app f u)[σ]ᵗ = app (B := B[scons (Γ := Γ,A[σ]) (σ ∘ p) q]) f[σ]ᵗ u[σ]ᵗ.
+Proof.
+  reflexivity.
+Qed.
+
+Lemma beta :
+  forall Γ A B (b : Tm (Γ, A) B) (u : Tm Γ A),
+    app (λ b) u = b[scons id u]ᵗ.
+Proof.
+  reflexivity.
+Qed.
+
+Lemma eta :
+  forall Γ A B (f : Tm Γ (Π A B)),
+    λ (app (B := B[scons (Γ := (Γ,A),A[p]) (p ∘ p) q]) f[p]ᵗ q) = f.
+Proof.
+  reflexivity.
+Qed.
+
+(* It supports a universe *)
+Definition U {Γ} : Ty Γ :=
+  fun γ => Type.
+
+Definition El {Γ} (a : Tm Γ U) : Ty Γ :=
+  fun γ => a γ.
+
+Definition π {Γ} (a : Tm Γ U) (b : Tm Γ (Π (El a) U)) : Tm Γ U :=
+  fun γ => forall (x : a γ), (b γ x).
+
+Lemma Usubs :
+  forall Γ Δ (σ : Subs Γ Δ),
+    U[σ] = U.
+Proof.
+  reflexivity.
+Qed.
+
+Lemma Elsubs :
+  forall Γ Δ (σ : Subs Γ Δ) (a : Tm Δ U),
+    (El a)[σ] = El a[σ]ᵗ.
+Proof.
+  reflexivity.
+Qed.
+
+Lemma Elπ :
+  forall Γ (a : Tm Γ U) (b : Tm Γ (Π (El a) U)),
+    El (π a b) = Π (El a) (El (app (B := U) b[p]ᵗ q)).
 Proof.
   reflexivity.
 Qed.
